src/mebi_help.ml
@@ -1,0 +1,201 @@
+open Logging
+
+type help_set_kind =
+  | General of unit
+  | Bound of int
+  | DumpToFile of unit
+  | ShowDebug of unit
+  | ShowDetails of unit
+  | WeakMode of unit
+  | Weak of unit
+
+type help_kind =
+  | Basic of unit
+  | Set of help_set_kind
+  | Check of unit
+  | LTS of unit
+  | FSM of unit
+  | Saturate of unit
+  | Minimize of unit
+  | Bisim of unit
+  | Info of unit
+  | Unrecognized of unit
+
+let show_instructions_to_toggle_weak (weak_mode : bool) : unit =
+  if weak_mode
+  then
+    Log.notice
+      "Checking for Weak Bisimilarity.\n\
+       To check for Strong Bisimilarity use the command \"MeBi Set WeakMode \
+       False\""
+  else
+    Log.notice
+      "Checking for Strong Bisimilarity (since weak mode is disabled)\n\
+       To Check for Weak Bisimilarity use the command \"MeBi Set WeakMode \
+       True\""
+;;
+
+let show_instructions_to_enable_weak () : unit =
+  Log.notice
+    "Weak mode is not currently enabled.\n\
+     Use the command \"MeBi Set WeakMode True\" to enable it (and \"MeBi Set \
+     WeakMode False\" to disable it).\n"
+;;
+
+let show_instructions_to_set_weak () : unit =
+  Log.notice
+    "Cannot saturate without any silent actions.\n\
+     Use the command \"MeBi Set Weak ...\" to specify how you are encoding \
+     silent transitions.\n\
+     For example:\n\
+    \  1) \"MeBi Set Weak Option nat\" is for labels of type \"option nat\", \
+     where silent actions are \"None\" and visible actions are \"Some _\"\n\
+    \  2) \"MeBi Set Weak TAU of ACTION\" is for labels of inductive type \
+     \"ACTION\" that has some constructor \"TAU\"\n"
+;;
+
+let show_help_basic () : unit =
+  Log.notice
+    "All commands for this plugin begin with \"MeBi\" and are followed one of \
+     the following:\n\
+     Set, Check, LTS, FSM, Saturate, Minimize, Bisim.\n\n\
+     Use the command \"MeBi Help x\" for more information\n\
+     (where x is one of the terms above)\n"
+;;
+
+let show_help_unrecognized_command () : unit =
+  Log.notice "Command not recognized.\n";
+  show_help_basic ()
+;;
+
+let show_help_set () : unit =
+  Log.notice
+    (Printf.sprintf
+       "Certain commands set parameters the plugin uses when running other \
+        commands.\n\
+        These parameters are: Bound, DumpToFile, ShowDebug, WeakMode, Weak\n\n\
+        Use the command \"MeBi Help Set x\" for more information\n\
+        (where x is one of the parameters above)\n")
+;;
+
+let show_help_set_bound (default_bound : int) : unit =
+  Log.notice
+    (Printf.sprintf
+       "Use the command \"MeBi Set Bound n\" to set the upper-bound of the \
+        number of unique states that can be reached when building the LTS from \
+        a coq term, where \"n\" is an natural integer number.\n\n\
+        Use command \"MeBi Set Bound Default\" to reset this to the default, \
+        which is: %i"
+       default_bound)
+;;
+
+let show_help_set_dump_to_file () : unit =
+  Log.notice
+    "Use the command \"MeBi Set DumpToFile True\" to enable the internal \
+     results (and/or models) of any command run to a (JSON) file.\n\
+     Disable this behaviour using \"MeBi Set DumpToFile False\"\n"
+;;
+
+let show_help_set_show_debug () : unit =
+  Log.notice
+    "Use the command \"MeBi Set ShowDebug True\" to enable debug messages.\n\
+     Disable them using \"MeBi Set ShowDebug False\"\n"
+;;
+
+let show_help_set_show_details () : unit =
+  Log.notice
+    "Use the command \"MeBi Set ShowDetails True\" to enable additional detail \
+     messages.\n\
+     Disable them using \"MeBi Set ShowDetails False\"\n"
+;;
+
+let show_help_set_weak_mode () : unit =
+  Log.notice
+    "Use the command \"MeBi Set WeakMode True\" to enable it (and \"MeBi \
+     WeakMode False\" to disable it).\n"
+;;
+
+let show_help_set_weak () : unit =
+  Log.notice
+    "Use the command \"MeBi Set Weak ...\" to specify how you are encoding \
+     silent transitions.\n\
+     For example:\n\
+    \  1) \"MeBi Set Weak Option nat\" is for labels of type \"option nat\", \
+     where silent actions are \"None\" and visible actions are \"Some _\"\n\
+    \  2) \"MeBi Set Weak TAU of ACTION\" is for labels of inductive type \
+     \"ACTION\" that has some constructor \"TAU\"\n"
+;;
+
+let show_help_check () : unit =
+  Log.notice
+    "Use the command \"MeBi Check x\" to see what any of Bound, DumpToFile, \
+     ShowDebug, WeakMode, Weak are set to.\n\
+     Use the command \"MeBi Check All\" to see for them all.\n"
+;;
+
+let show_help_lts () : unit = Log.notice "Use the command \"MeBi LTS ...\"\n"
+let show_help_fsm () : unit = Log.notice "Use the command \"MeBi FSM ...\"\n"
+
+let show_help_saturate () : unit =
+  Log.notice "Use the command \"MeBi Saturate ...\"\n"
+;;
+
+let show_help_minimize () : unit =
+  Log.notice "Use the command \"MeBi Minimize ...\"\n"
+;;
+
+let show_help_bisim () : unit =
+  Log.notice "Use the command \"MeBi Bisim ...\"\n"
+;;
+
+let show_help_info () : unit =
+  Log.notice
+    "Use the command \"MeBi Info\" to be shown information about the plugin, \
+     including a some guidelines and a list of limitations."
+;;
+
+let show_guidelines_and_limitations () : unit =
+  Log.notice
+    "Guidelines & Limitations\n\n\
+     - To construct the LTS from a term, the term must be an inductive type of \
+     the shape:\n\
+     \tterm -> label -> term -> Prop\n\
+     where \"term\" and \"label\" are defined elsewhere.\n\n\
+     - The \"label\" type must be of either Type or Set.\n\n\
+     - The plugin supports multi-layered LTS definitions, where the \
+     constructors of the inductive type have premises that are either \
+     recursive or reference a different inductive LTS proposition type.\n\n\
+     - The premises of the constructors in the inductive LTS proposition types \
+     must only contain other propositions and not, e.g., equalities.\n\
+     In cases such as equality, you must simply \"inline\" it by substitution.\n\
+     For example, instead of writing:\n\
+     \tInductive lts : nat -> bool -> nat -> Prop :=\n\
+     \t| do_action : forall a t t', t' = some_fun t -> lts t a t'\n\n\
+     You must write:\n\
+     \tInductive lts : nat -> bool -> nat -> Prop :=\n\
+     \t| do_action : forall a t, lts t a (some_fun t)\n\n\
+     - \n\n\
+    \ TODO..."
+;;
+
+let handle_help (c : help_kind) : unit =
+  match c with
+  | Basic () -> show_help_basic ()
+  | Set s ->
+    (match s with
+     | General () -> show_help_set ()
+     | Bound b -> show_help_set_bound b
+     | DumpToFile () -> show_help_set_dump_to_file ()
+     | ShowDebug () -> show_help_set_show_debug ()
+     | ShowDetails () -> show_help_set_show_details ()
+     | WeakMode () -> show_help_set_weak_mode ()
+     | Weak () -> show_help_set_weak ())
+  | Check () -> show_help_check ()
+  | LTS () -> show_help_lts ()
+  | FSM () -> show_help_fsm ()
+  | Saturate () -> show_help_saturate ()
+  | Minimize () -> show_help_minimize ()
+  | Bisim () -> show_help_bisim ()
+  | Info () -> show_help_info ()
+  | Unrecognized () -> show_help_unrecognized_command ()
+;;
