src/mebi_help.mli
@@ -1,0 +1,42 @@
+type help_set_kind =
+  | General of unit
+  | Bound of int
+  | DumpToFile of unit
+  | ShowDebug of unit
+  | ShowDetails of unit
+  | WeakMode of unit
+  | Weak of unit
+
+type help_kind =
+  | Basic of unit
+  | Set of help_set_kind
+  | Check of unit
+  | LTS of unit
+  | FSM of unit
+  | Saturate of unit
+  | Minimize of unit
+  | Bisim of unit
+  | Info of unit
+  | Unrecognized of unit
+
+val show_instructions_to_toggle_weak : bool -> unit
+val show_instructions_to_enable_weak : unit -> unit
+val show_instructions_to_set_weak : unit -> unit
+val show_help_basic : unit -> unit
+val show_help_unrecognized_command : unit -> unit
+val show_help_set : unit -> unit
+val show_help_set_bound : int -> unit
+val show_help_set_dump_to_file : unit -> unit
+val show_help_set_show_debug : unit -> unit
+val show_help_set_show_details : unit -> unit
+val show_help_set_weak_mode : unit -> unit
+val show_help_set_weak : unit -> unit
+val show_help_check : unit -> unit
+val show_help_lts : unit -> unit
+val show_help_fsm : unit -> unit
+val show_help_saturate : unit -> unit
+val show_help_minimize : unit -> unit
+val show_help_bisim : unit -> unit
+val show_help_info : unit -> unit
+val show_guidelines_and_limitations : unit -> unit
+val handle_help : help_kind -> unit
